Move on_block out of StateTransition.

src/dafny/beacon/StateTransition.dfy
@@ -112,520 +112,206 @@ module StateTransition {
         // block_roots: VectorOfHistRoots,
         // state_roots: VectorOfHistRoots
     )
-
-    /**
-     *  The default block header.
-     */
-    const EMPTY_BLOCK_HEADER := BeaconBlockHeader(0 as Slot, EMPTY_BYTES32, EMPTY_BYTES32)
     
     /**
-     *  Genesis (initial) beacon state.
-     *  
-     *  @link{https://github.com/ethereum/eth2.0-specs/blob/dev/specs/phase0/beacon-chain.md#genesis-state}
+     *  Compute the state obtained after adding a block.
      */
-    const GENESIS_STATE := BeaconState(0, EMPTY_BLOCK_HEADER)
+    method stateTransition(s: BeaconState, b: BeaconBlockHeader) returns (s' : BeaconState)
+        //  make sure the last state was one right after addition of new block
+        // requires s.latest_block_header.state_root == EMPTY_BYTES32
+        //  a new block must be proposed for a slot that is later than s.slot
+        requires s.slot < b.slot
+        requires b.parent_root == hash_tree_root(forwardStateToSlot(resolveStateRoot(s), b.slot).latest_block_header) //    Req1
 
-    /**
-     *  Genesis block (header).
-     *
-     *  @link{https://github.com/ethereum/eth2.0-specs/blob/dev/specs/phase0/beacon-chain.md#genesis-block}
-     *  @note   In this simplified version blocks are same as headers.
-     */
-    const GENESIS_BLOCK_HEADER := BeaconBlockHeader(
-        0 as Slot,  
-        EMPTY_BYTES32 , 
-        hash_tree_root(GENESIS_STATE)
-    )
+        /** The store is not modified. */
+        // ensures store == old(store)
 
-    /**
-     *  The store recording the blocks and the states.
-     *  
-     *  @param  blocks          maps hash_tree_root(b) to b
-     *  @param  block_states    maps a Root (hash_tree_root of a block) to a state.
-     *
-     *  @note                   From the spec 
-     *  @link{https://github.com/ethereum/eth2.0-specs/blob/dev/specs/phase0/fork-choice.md#on_block}           
-     *  @todo                   It seems that blocks and block_states should have the same
-     *                          keys at any time. We may prove it.
-     */
-    datatype Store = Store (
-        blocks : map<Root, BeaconBlockHeader>,
-        block_states : map<Root, BeaconState>
-    )
+        /** The set of already ccepted blocks is not modified. */
+        // ensures acceptedBlocks == old(acceptedBlocks)
 
-    /**
-     *  This function is specialised for the genesis state.
-     *
-     *  @param  anchor_state    A state to be regarded as a trusted state, to not 
-     *                          roll back beyond. This should be the genesis state for a full client.
-     *  
-     *  @note                   The original code in python starts with:
-     *                          var anchor_block_header := anchor_state.latest_block_header;
-     *                          if (anchor_block_header.state_root == Bytes32()) {
-     *                              anchor_block_header.state_root := hash_tree_root(anchor_state)
-     *                          };
-     *                          It is here implemented by forcing the condition to be true.
-     *
-     *  @note                   [from specs] The block for anchor_root is incorrectly initialized 
-     *                          to the block 
-     *                          header, rather than the full block. This does not affect 
-     *                          functionality but will be cleaned up in subsequent releases.
-     *
-     *  @link{https://github.com/ethereum/eth2.0-specs/blob/dev/specs/phase0/fork-choice.md#get_forkchoice_store}
-     */
-    function method get_forkchoice_store(anchor_state: BeaconState) : Store 
-        requires anchor_state.latest_block_header.state_root == EMPTY_BYTES32
+        /** The next state latest_block_header is same as b except for state_root that is 0. */
+        ensures s'.latest_block_header == b.(state_root := EMPTY_BYTES32)
+
+        ensures s'.slot == b.slot
+
+        // modifies this
     {
-        var anchor_block_header := anchor_state.latest_block_header.(
-            state_root := hash_tree_root(anchor_state)
-        );
-        var anchor_root := hash_tree_root(anchor_block_header);
-        Store(
-            map[anchor_root := anchor_block_header],    // blocks
-            map[anchor_root := anchor_state]            //  block_states
-        )
-    }
+        //  finalise slots before b.slot
+        var s1 := processSlots(s, b.slot);
 
-    /**
-     *  The genesis store.
-     *
-     *  @link{https://github.com/ethereum/eth2.0-specs/blob/dev/specs/phase0/fork-choice.md#get_forkchoice_store}
-     */
-    const GENESIS_STORE := get_forkchoice_store(GENESIS_STATE)
+        //  Process block
+        s' := processBlock(s1, b);  
 
-    /**
-     *  Property of the genesis store.
-     */
-    lemma genesisStoreHasGenesisBlockAndState() 
-        ensures GENESIS_STORE == Store(
-            map[hash_tree_root(GENESIS_BLOCK_HEADER) := GENESIS_BLOCK_HEADER],
-            map[hash_tree_root(GENESIS_BLOCK_HEADER) := GENESIS_STATE]
-        )
-    {   //  Thanks Dafny
-    }
+        //  Validate state block
+    }  
 
-    
-    /**
-     *  A Beacon Chain environement i.e. with Store etc
-     */
-    class Env {
+/**
+    *  Advance current state to a given slot.
+    *
+    *  This mainly consists in advancing the slot number to
+    *  a target future `slot` number and updating/recording the history of intermediate
+    *  states (and block headers). 
+    *  Under normal circumstances, where a block is received at each slot,
+    *  this involves only one iteration of the loop.
+    *  Otherwise, the first iteration of the loop `finalises` the block header
+    *  of the previous slot before recortding it, 
+    *  and subsequent rounds advance the slot number and record the history of states
+    *  and blocks for each slot.
+    *
+    *  @param  s       A state
+    *  @param  slot    The slot to advance to. This is usually the slot of newly
+    *                  proposed block.
+    *  @returns        The state obtained after advancing the history to slot.
+    *      
+    *   @note          The specs have the the first processSlot integrated
+    *                  in the while loop. However, because s.slot < slot,
+    *                  the while bdoy must be executed at least one time.
+    *                  To simplify the proof, we have taken this first iteration
+    *                  outside of the loop. It does not change the semantics
+    *                  but enables us to use the state obtained after the first
+    *                  iteration the loop and prove it is the same as 
+    *                  resolveStateRoot(s); 
+    *
+    */
+    method processSlots(s: BeaconState, slot: Slot) returns (s' : BeaconState)
+        requires s.slot < slot  //  update in 0.12.0 (was <= before)
 
-        /**
-         *  The record of blocks that have been added to the chain.
-         *
-         *  The store.Keys contain the hash tree root of the corresponding store.Values.
-         */
-        var store : Store
-
-        /**
-         *  Track the set of blocks that have been added to the store.
-         */
-        ghost var acceptedBlocks : set<BeaconBlockHeader>
-
-        /**
-         *  Start with the genesis store and one accepted block, GENESIS_BLOCK_HEADER
-         */
-        constructor ()  
-
-            /** Trying to verify  storeInvariant2 generates boogie name error. */
-            // ensures storeInvariant2()
-            /** Verify storeInvariant2() manually. */
-            // ensures acceptedBlocks == {GENESIS_BLOCK_HEADER}
-            ensures hash_tree_root(GENESIS_BLOCK_HEADER) in store.block_states.Keys
-            // ensures hash_tree_root(GENESIS_BLOCK_HEADER) in store.blocks.Keys
-            ensures store.block_states[hash_tree_root(GENESIS_BLOCK_HEADER)].latest_block_header == GENESIS_BLOCK_HEADER.(state_root := EMPTY_BYTES32) 
-
-            //  for some reason removing the previous ensures creates a name resolution error in
-            //  Dafny.
-            ensures storeIsValid()
-            ensures storeInvariant4()
-            ensures storeInvariant5()
-
-        {  
-            store := GENESIS_STORE;
-            acceptedBlocks := { GENESIS_BLOCK_HEADER }; 
-        }
-
-        /** The keys in the store maps are in sync. */
-        predicate storeInvariant0() 
-            reads this
-        {
-            store.blocks.Keys == store.block_states.Keys 
-        }
-
-        /**
-         *  Every accepted block is in the store its key is is the hash_tree_root,
-         */
-        predicate storeInvariant1() 
-            reads this
-        {
-            forall b :: b in acceptedBlocks ==> 
-                hash_tree_root(b) in store.blocks.Keys 
-                && store.blocks[hash_tree_root(b)] == b
-        }
-
-        /** 
-         *  Every accepted block `b` has an associated state in block_states and
-         *  the corresponding state has a latest_block_header that is the block `b`
-         *  with its state_root field nullified.
-         */
-        predicate storeInvariant2() 
-            reads this 
-        {
-            forall b :: b in acceptedBlocks ==> 
-                hash_tree_root(b) in store.block_states.Keys 
-                && store.block_states[hash_tree_root(b)].latest_block_header == b.(state_root := EMPTY_BYTES32) 
-                // && store.block_states[hash_tree_root(b)].slot <= b.slot
-        }
-
-        /**
-         *  In this invariant it would be nice to have:
-         *   hash_tree_root(b) in keys ==> b in acceptedBlocks (or Values)
-         *  This would enable us to conclude that 
-         *              hash_tree_root(b) !in store.blocks.Keys from  b !in acceptedBlocks
-         *  and then we can omit
-         *              requires hash_tree_root(b) !in store.blocks.Keys
-         *  in on_block.
-         */
-        predicate storeInvariant3() 
-            reads this
-        {
-            acceptedBlocks == store.blocks.Values
-
-        }
-
-        predicate storeInvariant4() 
-            reads this
-        {
-            forall b :: b in acceptedBlocks && b != GENESIS_BLOCK_HEADER ==>
-                b.parent_root in store.blocks.Keys
-                && store.blocks[b.parent_root].slot < b.slot 
-        }
-
-        predicate storeInvariant5() 
-            reads this
-        {
-            forall b :: b in acceptedBlocks && b != GENESIS_BLOCK_HEADER ==>
-                b.parent_root in store.blocks.Keys
-                && b.parent_root in store.block_states.Keys
-                && store.blocks[b.parent_root].slot == store.block_states[b.parent_root].slot
-        }
-
-        // predicate coReachOfGenesisBlock(b: BeaconBlockHeader ) 
-        // {
-        //     if ( b == GENESIS_BLOCK_HEADER ) then   
-        //         true 
-        //     else 
-
-        // }
-
-        /**
-         *  Store is valid if all the invariants are satisfied,
-         */
-        predicate storeIsValid() 
-            reads this
-        {
-            true 
-            && storeInvariant0()
-            && storeInvariant1()
-            && storeInvariant2()
-            && storeInvariant3()
-        }
-
-        /**
-         *  @param  pre_state   The last beacon state that the block is supposed to attach to.
-         *                      This is not a real parameter as it is constrained to be
-         *                      the state that corresponds to the bloc parent_root but here
-         *                      for convenience and readability.
-         *  @param  b           A block to be added to the chain.
-         */
-        method on_block(b: BeaconBlockHeader, pre_state : BeaconState) 
-
-            requires storeIsValid()
-            requires storeInvariant4()
-            requires storeInvariant5()
-
-            /** @todo remove the next requires as it should follow from
-            the fact that b must have a slot > pre_state and thus cannot
-            be in blocks.Values and  its has cannot be in the keys. 
-            See invariant3().
-            */
-            requires b !in acceptedBlocks
-            requires hash_tree_root(b) !in store.blocks.Keys
-
-            requires b.parent_root in store.block_states
-
-            //  R1: set pre_state using the store
-            requires pre_state == store.block_states[b.parent_root]
-            //  R2: Necessary for process_slots to go ahead
-            requires pre_state.slot < b.slot
-
-            //  R3: it does not follow from R1 but is necessary to make sure
-            //  process_slots can go ahead.
-            //  It states that the block should be attached to a state that is obtained
-            //  by fast forwarding pre_state to the slot of `b`.
-            requires b.parent_root == hash_tree_root(forwardStateToSlot(resolveStateRoot(pre_state), b.slot).latest_block_header) 
-
-            ensures acceptedBlocks == old(acceptedBlocks) + { b };
-            ensures storeIsValid()
-            // ensures storeInvariant4()
-
-            modifies this
-
-
-        {
-            // assert(hash_tree_root(b) !in store.blocks.Keys);
-            // pre_state = store.block_states[block.parent_root].copy()
-            // Blocks cannot be in the future. If they are, their consideration must be delayed until the are in the past.
-            // assert get_current_slot(store) >= block.slot
-
-            // Add new block to the store
-            store := store.(blocks := store.blocks[hash_tree_root(b) := b] );
-            acceptedBlocks := acceptedBlocks + { b };
-
-            assert(b.parent_root in store.blocks.Keys);
-            assert(b.parent_root in store.block_states.Keys);
-            assert(store.block_states[b.parent_root].slot < b.slot);
-            assert(pre_state.slot < b.slot);    //  @todo remove requires
-            // assert(storeInvariant4());
-            // assert(store.blocks[b.parent_root].slot < b.slot);
-            // assert(storeInvariant4());
-
-            // Check that block is later than the finalized epoch slot (optimization to reduce calls to get_ancestor)
-            // finalized_slot = compute_start_slot_at_epoch(store.finalized_checkpoint.epoch)
-            // assert block.slot > finalized_slot
-            // Check block is a descendant of the finalized block at the checkpoint finalized slot
-            // assert get_ancestor(store, hash_tree_root(block), finalized_slot) == store.finalized_checkpoint.root
-
-
-            // assert(storeInvariant2());
-            // Check the block is valid and compute the post-state
-            var new_state := stateTransition(pre_state, b);
-           
-            assert(forall bb :: bb in acceptedBlocks && bb != GENESIS_BLOCK_HEADER && bb != b==>
-                bb.parent_root in store.blocks.Keys
-                && store.blocks[bb.parent_root].slot < bb.slot ) ;
-
-            // @todo need to prove invariant5 for the new block b only
-            assert(b.parent_root in store.blocks.Keys);
-
-            assert(pre_state.slot < b.slot);    //  @todo remove requires
-            assert(store.block_states[b.parent_root].slot == pre_state.slot);
-
-            // assert(storeInvariant4());
-            // Add new state for this block to the store
-            store := store.(block_states := store.block_states[hash_tree_root(b) := new_state] );
-            
-            assert(b.parent_root in store.blocks.Keys);
-            assert(b.parent_root in store.blocks.Keys);
-
-            // assert(new_state.slot == store.blocks[b.parent_root].slot);
-            assert(pre_state.slot < b.slot);    //  @todo remove requires
-            assert(store.block_states[b.parent_root].slot == pre_state.slot);
-            // assert(store.blocks[b.parent_root].slot < b.slot );
-
-        }
+        ensures s' == forwardStateToSlot( resolveStateRoot(s), slot)
+        // ensures store == old(store)
+        ensures s.latest_block_header.parent_root == s'.latest_block_header.parent_root  
         
-        /**
-         *  Compute the state obtained after adding a block.
-         */
-        method stateTransition(s: BeaconState, b: BeaconBlockHeader) returns (s' : BeaconState)
-            //  make sure the last state was one right after addition of new block
-            // requires s.latest_block_header.state_root == EMPTY_BYTES32
-            //  a new block must be proposed for a slot that is later than s.slot
-            requires s.slot < b.slot
-            requires b.parent_root == hash_tree_root(forwardStateToSlot(resolveStateRoot(s), b.slot).latest_block_header) //    Req1
+        /** The store is not modified. */
+        // ensures store == old(store)
 
-            /** The store is not modified. */
-            ensures store == old(store)
+        //  Termination ranking function
+        decreases slot - s.slot
+    {
+        //  Start from the current state and update it with processSlot.
+        //  First iteration of the loop in process_slots (Eth2)
+        s' := processSlot(s);
+        s':= s'.(slot := s'.slot + 1) ;
+        //  The following asserts are not needed for the proof but provided for readability. 
+        assert(s' == resolveStateRoot(s));  
+        //  s'.block header state_root should now be resolved
+        assert(s'.latest_block_header.state_root != EMPTY_BYTES32);
 
-            /** The set of already ccepted blocks is not modified. */
-            ensures acceptedBlocks == old(acceptedBlocks)
-
-            /** The next state latest_block_header is same as b except for state_root that is 0. */
-            ensures s'.latest_block_header == b.(state_root := EMPTY_BYTES32)
-
-            ensures s'.slot == b.slot
-
-            modifies this
+        //  Now fast forward to slot
+        //  Next iterations of process_slot (Eth2)
+        while (s'.slot < slot)  
+            invariant s'.slot <= slot
+            invariant s'.latest_block_header.state_root != EMPTY_BYTES32
+            invariant s' == forwardStateToSlot(resolveStateRoot(s), s'.slot) // Inv1
+            decreases slot - s'.slot 
         {
-            //  finalise slots before b.slot
-            var s1 := processSlots(s, b.slot);
+            s':= processSlot(s');
 
-            //  Process block
-            s' := processBlock(s1, b);  
-
-            //  Validate state block
-        }  
-
-        /**
-         *  Advance current state to a given slot.
-         *
-         *  This mainly consists in advancing the slot number to
-         *  a target future `slot` number and updating/recording the history of intermediate
-         *  states (and block headers). 
-         *  Under normal circumstances, where a block is received at each slot,
-         *  this involves only one iteration of the loop.
-         *  Otherwise, the first iteration of the loop `finalises` the block header
-         *  of the previous slot before recortding it, 
-         *  and subsequent rounds advance the slot number and record the history of states
-         *  and blocks for each slot.
-         *
-         *  @param  s       A state
-         *  @param  slot    The slot to advance to. This is usually the slot of newly
-         *                  proposed block.
-         *  @returns        The state obtained after advancing the history to slot.
-         *      
-         *   @note          The specs have the the first processSlot integrated
-         *                  in the while loop. However, because s.slot < slot,
-         *                  the while bdoy must be executed at least one time.
-         *                  To simplify the proof, we have taken this first iteration
-         *                  outside of the loop. It does not change the semantics
-         *                  but enables us to use the state obtained after the first
-         *                  iteration the loop and prove it is the same as 
-         *                  resolveStateRoot(s); 
-         *
-         */
-        method processSlots(s: BeaconState, slot: Slot) returns (s' : BeaconState)
-            requires s.slot < slot  //  update in 0.12.0 (was <= before)
-
-            ensures s' == forwardStateToSlot( resolveStateRoot(s), slot)
-            ensures store == old(store)
-            ensures s.latest_block_header.parent_root == s'.latest_block_header.parent_root  
-            
-            /** The store is not modified. */
-            ensures store == old(store)
-
-            //  Termination ranking function
-            decreases slot - s.slot
-        {
-            //  Start from the current state and update it with processSlot.
-            //  First iteration of the loop in process_slots (Eth2)
-            s' := processSlot(s);
+            //  s'.slot is now processed: history updated and block header resolved
+            //  The state's slot is processed and we can advance to the next slot.
             s':= s'.(slot := s'.slot + 1) ;
-            //  The following asserts are not needed for the proof but provided for readability. 
-            assert(s' == resolveStateRoot(s));  
-            //  s'.block header state_root should now be resolved
-            assert(s'.latest_block_header.state_root != EMPTY_BYTES32);
-
-            //  Now fast forward to slot
-            //  Next iterations of process_slot (Eth2)
-            while (s'.slot < slot)  
-                invariant s'.slot <= slot
-                invariant s'.latest_block_header.state_root != EMPTY_BYTES32
-                invariant s' == forwardStateToSlot(resolveStateRoot(s), s'.slot) // Inv1
-                decreases slot - s'.slot 
-            {
-                s':= processSlot(s');
-
-                //  s'.slot is now processed: history updated and block header resolved
-                //  The state's slot is processed and we can advance to the next slot.
-                s':= s'.(slot := s'.slot + 1) ;
-            }
-        }
-
-       /** 
-         *  Cache data for a slot.
-         *
-         *  This function also finalises the block header of the last block
-         *  so that it records the hash of the state `s`. 
-         *
-         *  @param  s   A state.
-         *  @returns    A new state where `s` has been added/cached to the history and
-         *              the block header tracks the hash of the most recent received
-         *              block.
-         *
-         *  @note       This function method could be a method (as per the Eth2 specs).
-         *              However, this requires to expose the properties of the computation
-         *              as methods are not inlined. 
-         *  @note       Matches eth2.0 specs, need to uncomment update of state/block_roots.
-         *
-         *  @todo       Make this a method to have a def closer to Eth2 implementation.  
-         */
-        method processSlot(s: BeaconState) returns (s' : BeaconState)
-            requires s.slot as nat + 1 < 0x10000000000000000 as nat
-
-            ensures  s.latest_block_header.state_root == EMPTY_BYTES32 ==>
-                s' == resolveStateRoot(s).(slot := s.slot)
-            ensures  s.latest_block_header.state_root != EMPTY_BYTES32 ==>
-                s' == nextSlot(s).(slot := s.slot)
-            ensures s.latest_block_header.parent_root == s'.latest_block_header.parent_root
-
-            /** The store is not modified. */
-            ensures store == old(store)
-        {
-            s' := s;
-
-            // Cache state root
-            //  Record the hash of the previous state in the history.
-            var previous_state_root := hash_tree_root(s); 
-
-            // s' := s'.(state_roots := s'.state_roots[(s'.slot % SLOTS_PER_HISTORICAL_ROOT) as int := previous_state_root]);
-
-            //  Cache latest block header state root
-            if (s'.latest_block_header.state_root == EMPTY_BYTES32) {
-                s' := s'.(latest_block_header := s'.latest_block_header.(state_root := previous_state_root));
-            }
-
-            //  Cache block root
-            var previous_block_root := hash_tree_root(s'.latest_block_header);
-
-            // s' := s'.(block_roots := s'.block_roots[(s.slot % SLOTS_PER_HISTORICAL_ROOT) as int := previous_block_root]);
-        }
-
-        /**
-         *  Verify that a block is valid.
-         *
-         *  @note   Matches eth2.0 specs, need to implement randao, eth1, operations. 
-         */
-        method processBlock(s: BeaconState, b: BeaconBlockHeader) returns (s' : BeaconState) 
-            requires b.slot == s.slot
-            requires b.parent_root == hash_tree_root(s.latest_block_header)
-
-            ensures s'.latest_block_header.parent_root == b.parent_root
-            ensures s'.latest_block_header == b.(state_root := EMPTY_BYTES32)
-            ensures s'.slot == s.slot
-
-            /** The store is not modified. */
-            ensures store == old(store)
-        {
-            //  Start by creating a block header from the ther actual block.
-            s' := processBlockHeader(s, b); 
-            
-            //  process_randao(s, b.body)
-            //  process_eth1_data(s, b.body)
-            //  process_operations(s, b.body)
-        }
-
-       /**
-         *  Check whether a block is valid and prepare and initialise new state
-         *  with a corresponding block header. 
-         *
-         *  @note   Matches eth2.0 specs except proposer slashing verification
-         */
-        method processBlockHeader(s: BeaconState, b: BeaconBlockHeader) returns (s' : BeaconState) 
-            //  Verify that the slots match
-            requires b.slot == s.slot  
-            // Verify that the parent matches
-            requires b.parent_root == hash_tree_root(s.latest_block_header) 
-
-            ensures s'.latest_block_header == b.(state_root := EMPTY_BYTES32)
-            ensures s'.latest_block_header.parent_root == b.parent_root
-            ensures s'.slot == s.slot
-
-            /** The store is not modified. */
-            ensures store == old(store)
-        {
-            s':= s.(
-                latest_block_header := BeaconBlockHeader(
-                    b.slot,
-                    b.parent_root,
-                    EMPTY_BYTES32
-                )
-            );
         }
     }
 
+    /** 
+     *  Cache data for a slot.
+     *
+     *  This function also finalises the block header of the last block
+     *  so that it records the hash of the state `s`. 
+     *
+     *  @param  s   A state.
+     *  @returns    A new state where `s` has been added/cached to the history and
+     *              the block header tracks the hash of the most recent received
+     *              block.
+     *
+     *  @note       This function method could be a method (as per the Eth2 specs).
+     *              However, this requires to expose the properties of the computation
+     *              as methods are not inlined. 
+     *  @note       Matches eth2.0 specs, need to uncomment update of state/block_roots.
+     *
+     *  @todo       Make this a method to have a def closer to Eth2 implementation.  
+     */
+    method processSlot(s: BeaconState) returns (s' : BeaconState)
+        requires s.slot as nat + 1 < 0x10000000000000000 as nat
+
+        ensures  s.latest_block_header.state_root == EMPTY_BYTES32 ==>
+            s' == resolveStateRoot(s).(slot := s.slot)
+        ensures  s.latest_block_header.state_root != EMPTY_BYTES32 ==>
+            s' == nextSlot(s).(slot := s.slot)
+        ensures s.latest_block_header.parent_root == s'.latest_block_header.parent_root
+
+        /** The store is not modified. */
+        // ensures store == old(store)
+    {
+        s' := s;
+
+        // Cache state root
+        //  Record the hash of the previous state in the history.
+        var previous_state_root := hash_tree_root(s); 
+
+        // s' := s'.(state_roots := s'.state_roots[(s'.slot % SLOTS_PER_HISTORICAL_ROOT) as int := previous_state_root]);
+
+        //  Cache latest block header state root
+        if (s'.latest_block_header.state_root == EMPTY_BYTES32) {
+            s' := s'.(latest_block_header := s'.latest_block_header.(state_root := previous_state_root));
+        }
+
+        //  Cache block root
+        var previous_block_root := hash_tree_root(s'.latest_block_header);
+
+        // s' := s'.(block_roots := s'.block_roots[(s.slot % SLOTS_PER_HISTORICAL_ROOT) as int := previous_block_root]);
+    }
+
+    /**
+     *  Verify that a block is valid.
+     *
+     *  @note   Matches eth2.0 specs, need to implement randao, eth1, operations. 
+     */
+    method processBlock(s: BeaconState, b: BeaconBlockHeader) returns (s' : BeaconState) 
+        requires b.slot == s.slot
+        requires b.parent_root == hash_tree_root(s.latest_block_header)
+
+        ensures s'.latest_block_header.parent_root == b.parent_root
+        ensures s'.latest_block_header == b.(state_root := EMPTY_BYTES32)
+        ensures s'.slot == s.slot
+
+        /** The store is not modified. */
+        // ensures store == old(store)
+    {
+        //  Start by creating a block header from the ther actual block.
+        s' := processBlockHeader(s, b); 
+        
+        //  process_randao(s, b.body)
+        //  process_eth1_data(s, b.body)
+        //  process_operations(s, b.body)
+    }
+
+    /**
+     *  Check whether a block is valid and prepare and initialise new state
+     *  with a corresponding block header. 
+     *
+     *  @note   Matches eth2.0 specs except proposer slashing verification
+     */
+    method processBlockHeader(s: BeaconState, b: BeaconBlockHeader) returns (s' : BeaconState) 
+        //  Verify that the slots match
+        requires b.slot == s.slot  
+        // Verify that the parent matches
+        requires b.parent_root == hash_tree_root(s.latest_block_header) 
+
+        ensures s'.latest_block_header == b.(state_root := EMPTY_BYTES32)
+        ensures s'.latest_block_header.parent_root == b.parent_root
+        ensures s'.slot == s.slot
+
+        /** The store is not modified. */
+        // ensures store == old(store)
+    {
+        s':= s.(
+            latest_block_header := BeaconBlockHeader(
+                b.slot,
+                b.parent_root,
+                EMPTY_BYTES32
+            )
+        );
+    }
+    
     //  Specifications of finalisation of a state and forward to future slot.
 
     /**
