src/dafny/beacon/ForkChoice.dfy
@@ -1,0 +1,350 @@
+/*
+ * Copyright 2020 ConsenSys AG.
+ *
+ * Licensed under the Apache License, Version 2.0 (the "License"); you may 
+ * not use this file except in compliance with the License. You may obtain 
+ * a copy of the License at http://www.apache.org/licenses/LICENSE-2.0
+ *
+ * Unless required by applicable law or agreed to in writing, software dis-
+ * tributed under the License is distributed on an "AS IS" BASIS, WITHOUT 
+ * WARRANTIES OR CONDITIONS OF ANY KIND, either express or implied. See the 
+ * License for the specific language governing permissions and limitations 
+ * under the License.
+ */
+
+include "../ssz/Constants.dfy"
+include "../utils/NativeTypes.dfy"
+include "../utils/Eth2Types.dfy"
+include "../ssz/Constants.dfy"
+include "../utils/Helpers.dfy"
+include "Validators.dfy"
+include "BeaconChain.dfy"
+include "StateTransition.dfy"
+
+/**
+ * Fork choice rule for the Beacon Chain.
+ */
+module FirkChoice {
+    
+    //  Import some constants and types
+    import opened NativeTypes
+    import opened Eth2Types
+    import opened Constants
+    import opened BeaconChain
+    import opened StateTransition
+    import opened Helpers
+
+    /**
+     *  The default block header.
+     */
+    const EMPTY_BLOCK_HEADER := BeaconBlockHeader(0 as Slot, EMPTY_BYTES32, EMPTY_BYTES32)
+    
+    /**
+     *  Genesis (initial) beacon state.
+     *  
+     *  @link{https://github.com/ethereum/eth2.0-specs/blob/dev/specs/phase0/beacon-chain.md#genesis-state}
+     */
+    const GENESIS_STATE := BeaconState(0, EMPTY_BLOCK_HEADER)
+
+    /**
+     *  Genesis block (header).
+     *
+     *  @link{https://github.com/ethereum/eth2.0-specs/blob/dev/specs/phase0/beacon-chain.md#genesis-block}
+     *  @note   In this simplified version blocks are same as headers.
+     */
+    const GENESIS_BLOCK_HEADER := BeaconBlockHeader(
+        0 as Slot,  
+        EMPTY_BYTES32 , 
+        hash_tree_root(GENESIS_STATE)
+    )
+
+    /**
+     *  The store recording the blocks and the states.
+     *  
+     *  @param  blocks          maps hash_tree_root(b) to b
+     *  @param  block_states    maps a Root (hash_tree_root of a block) to a state.
+     *
+     *  @note                   From the spec 
+     *  @link{https://github.com/ethereum/eth2.0-specs/blob/dev/specs/phase0/fork-choice.md#on_block}           
+     *  @todo                   It seems that blocks and block_states should have the same
+     *                          keys at any time. We may prove it.
+     */
+    datatype Store = Store (
+        blocks : map<Root, BeaconBlockHeader>,
+        block_states : map<Root, BeaconState>
+    )
+
+    /**
+     *  This function is specialised for the genesis state.
+     *
+     *  @param  anchor_state    A state to be regarded as a trusted state, to not 
+     *                          roll back beyond. This should be the genesis state for a full client.
+     *  
+     *  @note                   The original code in python starts with:
+     *                          var anchor_block_header := anchor_state.latest_block_header;
+     *                          if (anchor_block_header.state_root == Bytes32()) {
+     *                              anchor_block_header.state_root := hash_tree_root(anchor_state)
+     *                          };
+     *                          It is here implemented by forcing the condition to be true.
+     *
+     *  @note                   [from specs] The block for anchor_root is incorrectly initialized 
+     *                          to the block 
+     *                          header, rather than the full block. This does not affect 
+     *                          functionality but will be cleaned up in subsequent releases.
+     *
+     *  @link{https://github.com/ethereum/eth2.0-specs/blob/dev/specs/phase0/fork-choice.md#get_forkchoice_store}
+     */
+    function method get_forkchoice_store(anchor_state: BeaconState) : Store 
+        requires anchor_state.latest_block_header.state_root == EMPTY_BYTES32
+    {
+        var anchor_block_header := anchor_state.latest_block_header.(
+            state_root := hash_tree_root(anchor_state)
+        );
+        var anchor_root := hash_tree_root(anchor_block_header);
+        Store(
+            map[anchor_root := anchor_block_header],    // blocks
+            map[anchor_root := anchor_state]            //  block_states
+        )
+    }
+
+    /**
+     *  The genesis store.
+     *
+     *  @link{https://github.com/ethereum/eth2.0-specs/blob/dev/specs/phase0/fork-choice.md#get_forkchoice_store}
+     */
+    const GENESIS_STORE := get_forkchoice_store(GENESIS_STATE)
+
+    /**
+     *  Property of the genesis store.
+     */
+    lemma genesisStoreHasGenesisBlockAndState() 
+        ensures GENESIS_STORE == Store(
+            map[hash_tree_root(GENESIS_BLOCK_HEADER) := GENESIS_BLOCK_HEADER],
+            map[hash_tree_root(GENESIS_BLOCK_HEADER) := GENESIS_STATE]
+        )
+    {   //  Thanks Dafny
+    }
+
+    /**
+     *  A Beacon Chain environement i.e. with Store etc
+     */
+    class Env {
+
+        /**
+         *  The record of blocks that have been added to the chain.
+         *
+         *  The store.Keys contain the hash tree root of the corresponding store.Values.
+         */
+        var store : Store
+
+        /**
+         *  Track the set of blocks that have been added to the store.
+         */
+        ghost var acceptedBlocks : set<BeaconBlockHeader>
+
+        /**
+         *  Start with the genesis store and one accepted block, GENESIS_BLOCK_HEADER
+         */
+        constructor ()  
+
+            /** Trying to verify  storeInvariant2 generates boogie name error. */
+            // ensures storeInvariant2()
+            /** Verify storeInvariant2() manually. */
+            // ensures acceptedBlocks == {GENESIS_BLOCK_HEADER}
+            ensures hash_tree_root(GENESIS_BLOCK_HEADER) in store.block_states.Keys
+            // ensures hash_tree_root(GENESIS_BLOCK_HEADER) in store.blocks.Keys
+            ensures store.block_states[hash_tree_root(GENESIS_BLOCK_HEADER)].latest_block_header == GENESIS_BLOCK_HEADER.(state_root := EMPTY_BYTES32) 
+
+            //  for some reason removing the previous ensures creates a name resolution error in
+            //  Dafny.
+            ensures storeIsValid()
+            ensures storeInvariant4()
+            ensures storeInvariant5()
+
+        {  
+            store := GENESIS_STORE;
+            acceptedBlocks := { GENESIS_BLOCK_HEADER }; 
+        }
+
+        /** The keys in the store maps are in sync. */
+        predicate storeInvariant0() 
+            reads this
+        {
+            store.blocks.Keys == store.block_states.Keys 
+        }
+
+        /**
+         *  Every accepted block is in the store its key is is the hash_tree_root,
+         */
+        predicate storeInvariant1() 
+            reads this
+        {
+            forall b :: b in acceptedBlocks ==> 
+                hash_tree_root(b) in store.blocks.Keys 
+                && store.blocks[hash_tree_root(b)] == b
+        }
+
+        /** 
+         *  Every accepted block `b` has an associated state in block_states and
+         *  the corresponding state has a latest_block_header that is the block `b`
+         *  with its state_root field nullified.
+         */
+        predicate storeInvariant2() 
+            reads this 
+        {
+            forall b :: b in acceptedBlocks ==> 
+                hash_tree_root(b) in store.block_states.Keys 
+                && store.block_states[hash_tree_root(b)].latest_block_header == b.(state_root := EMPTY_BYTES32) 
+                // && store.block_states[hash_tree_root(b)].slot <= b.slot
+        }
+
+        /**
+         *  In this invariant it would be nice to have:
+         *   hash_tree_root(b) in keys ==> b in acceptedBlocks (or Values)
+         *  This would enable us to conclude that 
+         *              hash_tree_root(b) !in store.blocks.Keys from  b !in acceptedBlocks
+         *  and then we can omit
+         *              requires hash_tree_root(b) !in store.blocks.Keys
+         *  in on_block.
+         */
+        predicate storeInvariant3() 
+            reads this
+        {
+            acceptedBlocks == store.blocks.Values
+
+        }
+
+        predicate storeInvariant4() 
+            reads this
+        {
+            forall b :: b in acceptedBlocks && b != GENESIS_BLOCK_HEADER ==>
+                b.parent_root in store.blocks.Keys
+                && store.blocks[b.parent_root].slot < b.slot 
+        }
+
+        predicate storeInvariant5() 
+            reads this
+        {
+            forall b :: b in acceptedBlocks && b != GENESIS_BLOCK_HEADER ==>
+                b.parent_root in store.blocks.Keys
+                && b.parent_root in store.block_states.Keys
+                && store.blocks[b.parent_root].slot == store.block_states[b.parent_root].slot
+        }
+
+        // predicate coReachOfGenesisBlock(b: BeaconBlockHeader ) 
+        // {
+        //     if ( b == GENESIS_BLOCK_HEADER ) then   
+        //         true 
+        //     else 
+
+        // }
+
+        /**
+         *  Store is valid if all the invariants are satisfied,
+         */
+        predicate storeIsValid() 
+            reads this
+        {
+            true 
+            && storeInvariant0()
+            && storeInvariant1()
+            && storeInvariant2()
+            && storeInvariant3()
+        }
+
+        /**
+         *  @param  pre_state   The last beacon state that the block is supposed to attach to.
+         *                      This is not a real parameter as it is constrained to be
+         *                      the state that corresponds to the bloc parent_root but here
+         *                      for convenience and readability.
+         *  @param  b           A block to be added to the chain.
+         */
+        method on_block(b: BeaconBlockHeader, pre_state : BeaconState) 
+
+            requires storeIsValid()
+            requires storeInvariant4()
+            requires storeInvariant5()
+
+            /** @todo remove the next requires as it should follow from
+            the fact that b must have a slot > pre_state and thus cannot
+            be in blocks.Values and  its has cannot be in the keys. 
+            See invariant3().
+            */
+            requires b !in acceptedBlocks
+            requires hash_tree_root(b) !in store.blocks.Keys
+
+            requires b.parent_root in store.block_states
+
+            //  R1: set pre_state using the store
+            requires pre_state == store.block_states[b.parent_root]
+            //  R2: Necessary for process_slots to go ahead
+            requires pre_state.slot < b.slot
+
+            //  R3: it does not follow from R1 but is necessary to make sure
+            //  process_slots can go ahead.
+            //  It states that the block should be attached to a state that is obtained
+            //  by fast forwarding pre_state to the slot of `b`.
+            requires b.parent_root == hash_tree_root(forwardStateToSlot(resolveStateRoot(pre_state), b.slot).latest_block_header) 
+
+            ensures acceptedBlocks == old(acceptedBlocks) + { b };
+            ensures storeIsValid()
+            // ensures storeInvariant4()
+
+            modifies this
+
+
+        {
+            // assert(hash_tree_root(b) !in store.blocks.Keys);
+            // pre_state = store.block_states[block.parent_root].copy()
+            // Blocks cannot be in the future. If they are, their consideration must be delayed until the are in the past.
+            // assert get_current_slot(store) >= block.slot
+
+            // Add new block to the store
+            store := store.(blocks := store.blocks[hash_tree_root(b) := b] );
+            acceptedBlocks := acceptedBlocks + { b };
+
+            assert(b.parent_root in store.blocks.Keys);
+            assert(b.parent_root in store.block_states.Keys);
+            assert(store.block_states[b.parent_root].slot < b.slot);
+            assert(pre_state.slot < b.slot);    //  @todo remove requires
+            // assert(storeInvariant4());
+            // assert(store.blocks[b.parent_root].slot < b.slot);
+            // assert(storeInvariant4());
+
+            // Check that block is later than the finalized epoch slot (optimization to reduce calls to get_ancestor)
+            // finalized_slot = compute_start_slot_at_epoch(store.finalized_checkpoint.epoch)
+            // assert block.slot > finalized_slot
+            // Check block is a descendant of the finalized block at the checkpoint finalized slot
+            // assert get_ancestor(store, hash_tree_root(block), finalized_slot) == store.finalized_checkpoint.root
+
+
+            // assert(storeInvariant2());
+            // Check the block is valid and compute the post-state
+            var new_state := stateTransition(pre_state, b);
+           
+            assert(forall bb :: bb in acceptedBlocks && bb != GENESIS_BLOCK_HEADER && bb != b==>
+                bb.parent_root in store.blocks.Keys
+                && store.blocks[bb.parent_root].slot < bb.slot ) ;
+
+            // @todo need to prove invariant5 for the new block b only
+            assert(b.parent_root in store.blocks.Keys);
+
+            assert(pre_state.slot < b.slot);    //  @todo remove requires
+            assert(store.block_states[b.parent_root].slot == pre_state.slot);
+
+            // assert(storeInvariant4());
+            // Add new state for this block to the store
+            store := store.(block_states := store.block_states[hash_tree_root(b) := new_state] );
+            
+            assert(b.parent_root in store.blocks.Keys);
+            assert(b.parent_root in store.blocks.Keys);
+
+            // assert(new_state.slot == store.blocks[b.parent_root].slot);
+            assert(pre_state.slot < b.slot);    //  @todo remove requires
+            assert(store.block_states[b.parent_root].slot == pre_state.slot);
+            // assert(store.blocks[b.parent_root].slot < b.slot );
+
+        }
+        
+    }
+}
